hip_graphmark.v
@@ -9,6 +9,7 @@ Module Type Mgraphmark.
   Parameter star : formula -> formula -> formula.
   Parameter and : formula -> formula -> formula.
   Parameter imp : formula -> formula -> formula.
+  Parameter ext : (nat -> formula) -> formula.
   Parameter not : formula -> formula.
   Parameter eq : node -> node -> formula.
   Parameter mwand : formula -> formula -> formula.
@@ -25,7 +26,7 @@ Module Type Mgraphmark.
   Axiom axiom_4 : forall v G1 G2 G G3 x l r, valid (imp (and (lookup G x v l r) (and (mark G l G1) (and (neq v 1) (and (mark G1 r G2) (update G2 x 1 l r G3))))) (and (mark G x G3) (lookup G3 x 1 l r))).
   Axiom axiom_5 : forall v G1 G2 G G3 x l r, valid (imp (and (lookup G x v l r) (and (update G x 1 l r G1) (and (neq v 1) (and (mark G1 r G2) (mark G2 l G3))))) (and (mark G x G3) (lookup G3 x 1 l r))).
   Axiom axiom_6 : forall v G1 G2 G G3 x l r, valid (imp (and (lookup G x v l r) (and (update G x 1 l r G1) (and (neq v 1) (and (mark G1 l G2) (mark G2 r G3))))) (and (mark G x G3) (lookup G3 x 1 l r))).
-  Axiom axiom_7 : forall v G x G1 y v1 l r, valid (imp (and (mark G x G1) (lookup G y v l r)) (and (subset_reach G x G1) (and (eq_notreach G x G1) (lookup G1 y v1 l r)))).
+  Axiom axiom_7 : forall v G x G1 y l r, valid (imp (and (mark G x G1) (lookup G y v l r)) (and (subset_reach G x G1) (and (eq_notreach G x G1) (ext (fun Anon_15 => (lookup G1 y Anon_15 l r)))))).
   Axiom axiom_8 : forall l r x G, valid (imp (lookup G x 1 l r) (mark G x G)).
   Axiom axiom_9 : forall G, valid (mark G null_node G).
   Axiom lem_subgraphupdate_l : forall G v G1 x v1 l r, valid (imp (and (star (graph l G1) (mwand (graph l G) (union (ptto_node x v l r) (union (graph l G) (graph r G))))) (and (subset_reach G l G1) (and (eq_notreach G l G1) (and (lookup G x v l r) (lookup G1 x v1 l r))))) (union (ptto_node x v1 l r) (union (graph l G1) (graph r G1)))).
